theories/VLSM/Core/VLSMProjections/VLSMStutteringEmbedding.v
@@ -1,0 +1,764 @@
+From Cdcl Require Import Itauto. #[local] Tactic Notation "itauto" := itauto auto.
+From stdpp Require Import prelude.
+From VLSM.Lib Require Import Preamble ListExtras StreamExtras StreamFilters StdppExtras.
+From VLSM.Core Require Import VLSM VLSMProjections.VLSMPartialProjection.
+
+(** * VLSM Stuttering Embeddings
+
+  Stuttering embeddings are VLSM projections guaranteeing the existence of
+  translations for all states and traces, in which a transition in the source
+  VLSM translates to a (possibly empty) sequence of transitions in the target VLSM.
+
+  A stuttering embedding is established from VLSM <<X>> to VLSM <<Y>>
+  (sharing the same messages) if there exists maps <<state_project>>
+  taking <<X>>-states to <<Y>>-states, and <<transition_item_project>>, taking
+  a transition from <<X>> to a list of transitions in <<Y>>, such that:
+
+  - [transition_item_project_consistency]: the state-translation of the destination
+    of a transition is the final state of the translation of the transition.
+  - [stuttering_embedding_preserves_valid_trace]s: traces obtained by
+    concatenating the translations of transition of a valid trace are valid.
+
+  An example of proper stuttering embedding is given by a VLSM summarizing the
+  transitions of another VLSM.
+*)
+
+Section sec_pre_definitions.
+
+Context
+  {message : Type}
+  {TX TY : VLSMType message}
+  (state_project : @state _ TX -> @state _ TY)
+  (transition_item_project : @transition_item _ TX -> list (@transition_item _ TY))
+  .
+
+Definition pre_VLSM_stuttering_embedding_finite_trace_project :
+  list (@transition_item _ TX) -> list (@transition_item _ TY) :=
+    mbind transition_item_project.
+
+Definition pre_VLSM_stuttering_embedding_infinite_trace_project
+  (s : Streams.Stream (@transition_item _ TX))
+  (Hs : InfinitelyOften (fun item => transition_item_project item <> []) s)
+  : Streams.Stream (@transition_item _ TY) :=
+  stream_concat_map transition_item_project s Hs.
+
+Definition pre_VLSM_stuttering_embedding_infinite_finite_trace_project
+  (s : Streams.Stream (@transition_item _ TX))
+  (Hs : FinitelyManyBound (fun item => transition_item_project item <> []) s)
+  : list (@transition_item _ TY) :=
+  bounded_stream_concat_map transition_item_project s Hs.
+
+Definition pre_VLSM_stuttering_embedding_finite_trace_project_app :
+  forall (l1 l2 : list (@transition_item _ TX)),
+    pre_VLSM_stuttering_embedding_finite_trace_project (l1 ++ l2)
+      =
+    pre_VLSM_stuttering_embedding_finite_trace_project l1
+      ++ pre_VLSM_stuttering_embedding_finite_trace_project l2
+  := mbind_app _.
+
+Lemma elem_of_pre_VLSM_stuttering_embedding_finite_trace_project :
+  forall (trX : list (@transition_item _ TX)) (itemY : @transition_item _ TY),
+    itemY ∈ pre_VLSM_stuttering_embedding_finite_trace_project trX
+      <->
+    exists (itemX : @transition_item _ TX), itemY ∈ transition_item_project itemX ∧ itemX ∈ trX.
+Proof. by intros; apply elem_of_list_bind. Qed.
+
+End sec_pre_definitions.
+
+Record VLSM_stuttering_embedding_type
+  {message : Type}
+  (X : VLSM message)
+  (TY : VLSMType message)
+  (state_project : vstate X -> @state _ TY)
+  (transition_item_project : vtransition_item X -> list (@transition_item _ TY))
+  : Prop :=
+{
+  transition_item_project_consistency :
+    forall sX itemX,
+      input_valid_transition_item X sX itemX ->
+        finite_trace_last (state_project sX) (transition_item_project itemX)
+          =
+        state_project (destination itemX);
+}.
+
+(** ** Stuttering embedding definitions and properties *)
+
+Section sec_stuttering_embedding_type_properties.
+
+Definition strong_transition_item_project_consistency
+  {message : Type}
+  [X : VLSM message]
+  [TY : VLSMType message]
+  (state_project : vstate X -> @state _ TY)
+  (transition_item_project : vtransition_item X -> list (@transition_item _ TY))
+  : Prop :=
+  forall sX lX inputX destinationX outputX,
+    vtransition X lX (sX, inputX) = (destinationX, outputX) ->
+    finite_trace_last (state_project sX)
+      (transition_item_project
+        {| l := lX; input := inputX; destination := destinationX; output := outputX|})
+      =
+    state_project destinationX.
+
+Section sec_pre_properties.
+
+Context
+  {message : Type}
+  (X : VLSM message)
+  (TY : VLSMType message)
+  (state_project : vstate X -> @state _ TY)
+  (transition_item_project : vtransition_item X -> list (@transition_item _ TY))
+  (Hsimul : VLSM_stuttering_embedding_type X TY state_project transition_item_project)
+  .
+
+Definition pre_VLSM_stuttering_embedding_finite_trace_last :
+  forall (s : vstate X) (tr : list (vtransition_item X)),
+    finite_valid_trace_from X s tr ->
+    finite_trace_last (state_project s)
+      (pre_VLSM_stuttering_embedding_finite_trace_project transition_item_project tr)
+      =
+    state_project (finite_trace_last s tr).
+Proof.
+  induction 1 using finite_valid_trace_from_rev_ind; [done |].
+  erewrite finite_trace_last_is_last,
+    pre_VLSM_stuttering_embedding_finite_trace_project_app,
+    finite_trace_last_app, IHfinite_valid_trace_from,
+    <- transition_item_project_consistency; [| done..].
+  by cbn; rewrite app_nil_r.
+Qed.
+
+End sec_pre_properties.
+
+Definition VLSM_partial_trace_project_from_stuttering_embedding
+  {message : Type}
+  {X : VLSM message}
+  {TY : VLSMType message}
+  (state_project : vstate X -> @state _ TY)
+  (transition_item_project : vtransition_item X -> list (@transition_item _ TY))
+  (trace_project := pre_VLSM_stuttering_embedding_finite_trace_project transition_item_project)
+  (str : vstate X * list (vtransition_item X))
+  : option (@state _ TY * list (@transition_item _ TY)) :=
+    let (s, tr) := str in Some (state_project s, trace_project tr).
+
+Context
+  {message : Type}
+  {X Y : VLSM message}
+  (state_project : vstate X -> vstate Y)
+  (transition_item_project : vtransition_item X -> list (vtransition_item Y))
+  (Hsimul : VLSM_stuttering_embedding_type X (type Y) state_project transition_item_project)
+  .
+
+(**
+  Any [VLSM_stuttering_embedding_type] determines a [VLSM_partial_projection_type],
+  allowing us to lift to VLSM stuttering embeddings the generic results proved
+  about VLSM partial projections.
+*)
+Lemma VLSM_partial_projection_type_from_stuttering_embedding :
+  VLSM_partial_projection_type X Y
+    (VLSM_partial_trace_project_from_stuttering_embedding state_project transition_item_project).
+Proof.
+  constructor; intros * Hpr * Hlst Htr.
+  apply Some_inj, pair_equal_spec in Hpr as [<- <-]; cbn.
+  rewrite pre_VLSM_stuttering_embedding_finite_trace_project_app.
+  eexists (state_project s'X), _.
+  split; [done |].
+  apply finite_valid_trace_from_app_iff in Htr as [].
+  by erewrite pre_VLSM_stuttering_embedding_finite_trace_last, Hlst.
+Qed.
+
+End sec_stuttering_embedding_type_properties.
+
+Section sec_VLSM_stuttering_embedding_definitions.
+
+Context
+  {message : Type}
+  (X Y : VLSM message)
+  (state_project : vstate X -> vstate Y)
+  (transition_item_project : vtransition_item X -> list (vtransition_item Y))
+  (trace_project := pre_VLSM_stuttering_embedding_finite_trace_project transition_item_project)
+  .
+
+Definition stuttering_embedding_input_valid_transition_item_validity : Prop :=
+  forall s item,
+    input_valid_transition_item X s item ->
+    finite_valid_trace_from_to Y (state_project s) (state_project (destination item))
+      (transition_item_project item).
+
+(**
+  Similarly to the [VLSM_partial_projection] case we distinguish two types of
+  stuttering embeddings: [VLSM_weak_stuttering_embedding] and
+  [VLSM_stuttering_embedding], distinguished by the fact that the weak
+  embeddings are not required to preserve initial states.
+*)
+Record VLSM_weak_stuttering_embedding : Prop :=
+{
+  weak_stuttering_embedding_type :>
+    VLSM_stuttering_embedding_type X (type Y) state_project transition_item_project;
+  weak_stuttering_embedding_preserves_valid_trace :
+    forall sX trX,
+      finite_valid_trace_from X sX trX ->
+      finite_valid_trace_from Y (state_project sX) (trace_project trX);
+}.
+
+Record VLSM_stuttering_embedding : Prop :=
+{
+  stuttering_embedding_type :>
+    VLSM_stuttering_embedding_type X (type Y) state_project transition_item_project;
+  stuttering_embedding_preserves_valid_trace :
+    forall sX trX,
+      finite_valid_trace X sX trX -> finite_valid_trace Y (state_project sX) (trace_project trX);
+}.
+
+Definition weak_stuttering_embedding_initial_state_preservation : Prop :=
+  forall s : state,
+    vinitial_state_prop X s -> valid_state_prop Y (state_project s).
+
+Definition strong_stuttering_embedding_initial_state_preservation : Prop :=
+  forall s : state,
+    vinitial_state_prop X s -> vinitial_state_prop Y (state_project s).
+
+Lemma strong_stuttering_embedding_initial_state_preservation_weaken :
+  strong_stuttering_embedding_initial_state_preservation ->
+    weak_stuttering_embedding_initial_state_preservation.
+Proof.
+  intros Hstrong s Hs.
+  apply initial_state_is_valid.
+  by apply Hstrong.
+Qed.
+
+End sec_VLSM_stuttering_embedding_definitions.
+
+Section sec_weak_stuttering_embedding_properties.
+
+Context
+  {message : Type}
+  {X Y : VLSM message}
+  {state_project : vstate X -> vstate Y}
+  {transition_item_project : vtransition_item X -> list (vtransition_item Y)}
+  .
+
+Section sec_weak_stuttering_embedding_trace_projection_redefinitions.
+
+(**
+  Here we restate the <<pre_>> definitions above to depend on [VLSM_weak_stuttering_embedding]
+  and have their state and transition item projection functions implicit.
+*)
+
+Definition VLSM_weak_stuttering_embedding_finite_trace_project
+  (Hsimul : VLSM_weak_stuttering_embedding X Y state_project transition_item_project)
+  : list (vtransition_item X) -> list (vtransition_item Y)
+  := pre_VLSM_stuttering_embedding_finite_trace_project transition_item_project.
+
+Definition elem_of_VLSM_weak_stuttering_embedding
+  (Hsimul : VLSM_weak_stuttering_embedding X Y state_project transition_item_project)
+  := elem_of_pre_VLSM_stuttering_embedding_finite_trace_project transition_item_project.
+
+Definition VLSM_weak_stuttering_embedding_infinite_trace_project
+  (Hsimul : VLSM_weak_stuttering_embedding X Y state_project transition_item_project)
+  (s : Streams.Stream (vtransition_item X))
+  (Hinf : InfinitelyOften (fun item => transition_item_project item <> []) s)
+  : Streams.Stream (vtransition_item Y)
+  := pre_VLSM_stuttering_embedding_infinite_trace_project transition_item_project s Hinf.
+
+Definition VLSM_weak_stuttering_embedding_infinite_finite_trace_project
+  (Hsimul : VLSM_weak_stuttering_embedding X Y state_project transition_item_project)
+  (s : Streams.Stream (vtransition_item X))
+  (Hfin : FinitelyManyBound (fun item => transition_item_project item <> []) s)
+  : list (vtransition_item Y)
+  := pre_VLSM_stuttering_embedding_infinite_finite_trace_project transition_item_project s Hfin.
+
+End sec_weak_stuttering_embedding_trace_projection_redefinitions.
+
+(**
+  While for the above section, the [VLSM_weak_stuttering_embedding] was necessary
+  to be mentioned explicitly, in the following we make it part of the context.
+*)
+
+Context
+  (Hsimul : VLSM_weak_stuttering_embedding X Y state_project transition_item_project).
+
+Definition VLSM_weak_stuttering_embedding_finite_trace_project_app :
+  forall l1 l2,
+    VLSM_weak_stuttering_embedding_finite_trace_project Hsimul (l1 ++ l2)
+      =
+    VLSM_weak_stuttering_embedding_finite_trace_project Hsimul l1
+      ++ VLSM_weak_stuttering_embedding_finite_trace_project Hsimul l2
+  := pre_VLSM_stuttering_embedding_finite_trace_project_app transition_item_project.
+
+Definition VLSM_weak_stuttering_embedding_finite_trace_last :
+  forall sX trX,
+    finite_valid_trace_from X sX trX ->
+    finite_trace_last (state_project sX)
+      (VLSM_weak_stuttering_embedding_finite_trace_project Hsimul trX)
+      =
+    state_project (finite_trace_last sX trX)
+  := pre_VLSM_stuttering_embedding_finite_trace_last _ _ _ _ Hsimul.
+
+Definition VLSM_weak_stuttering_embedding_finite_valid_trace_from :
+  forall sX trX,
+    finite_valid_trace_from X sX trX ->
+    finite_valid_trace_from Y (state_project sX)
+      (VLSM_weak_stuttering_embedding_finite_trace_project Hsimul trX)
+  := weak_stuttering_embedding_preserves_valid_trace _ _ _ _ Hsimul.
+
+Lemma VLSM_weak_stuttering_embedding_infinite_valid_trace_from :
+  forall sX trX (Hinf : InfinitelyOften (fun item => transition_item_project item <> []) trX),
+    infinite_valid_trace_from X sX trX ->
+    infinite_valid_trace_from Y (state_project sX)
+      (VLSM_weak_stuttering_embedding_infinite_trace_project Hsimul trX Hinf).
+Proof.
+  intros sX trX Hinf HtrX.
+  apply infinite_valid_trace_from_prefix_rev.
+  intros n.
+  destruct (stream_concat_map_ex_prefix transition_item_project trX Hinf n)
+    as (m & suf & Hrew).
+  apply finite_valid_trace_from_app_iff with (ls' := suf).
+  setoid_rewrite <- Hrew.
+  by apply VLSM_weak_stuttering_embedding_finite_valid_trace_from,
+    infinite_valid_trace_from_prefix.
+Qed.
+
+Lemma VLSM_weak_stuttering_embedding_infinite_finite_valid_trace_from :
+  forall sX trX (Hfin : FinitelyManyBound (fun item => transition_item_project item <> []) trX),
+    infinite_valid_trace_from X sX trX ->
+    finite_valid_trace_from Y (state_project sX)
+      (VLSM_weak_stuttering_embedding_infinite_finite_trace_project Hsimul trX Hfin).
+Proof.
+  intros sX trX Hfin HtrX.
+  apply VLSM_weak_stuttering_embedding_finite_valid_trace_from.
+  by apply infinite_valid_trace_from_prefix with (n := `Hfin) in HtrX.
+Qed.
+
+(**
+  Any [VLSM_weak_stuttering_embedding] determines a [VLSM_weak_partial_projection],
+  allowing us to lift to weak stuttering embeddings the generic results proved
+  about weak partial projections.
+*)
+Lemma VLSM_weak_partial_projection_from_stuttering_embedding :
+  VLSM_weak_partial_projection X Y
+    (VLSM_partial_trace_project_from_stuttering_embedding state_project transition_item_project).
+Proof.
+  split.
+  - by apply VLSM_partial_projection_type_from_stuttering_embedding, Hsimul.
+  - cbn; intros sX trX sY trY [= <- <-].
+    by apply VLSM_weak_stuttering_embedding_finite_valid_trace_from.
+Qed.
+
+Lemma VLSM_weak_stuttering_embedding_valid_state :
+  forall sX,
+    valid_state_prop X sX -> valid_state_prop Y (state_project sX).
+Proof.
+  by intro sX; eapply VLSM_weak_partial_projection_valid_state;
+    [apply VLSM_weak_partial_projection_from_stuttering_embedding |].
+Qed.
+
+Lemma VLSM_weak_stuttering_embedding_finite_valid_trace_from_to :
+  forall sX s'X trX,
+    finite_valid_trace_from_to X sX s'X trX ->
+      finite_valid_trace_from_to Y (state_project sX) (state_project s'X)
+        (VLSM_weak_stuttering_embedding_finite_trace_project Hsimul trX).
+Proof.
+  intros sX s'X trX HtrX.
+  apply valid_trace_add_last.
+  - eapply VLSM_weak_partial_projection_finite_valid_trace_from.
+    + by apply VLSM_weak_partial_projection_from_stuttering_embedding.
+    + done.
+    + by eapply valid_trace_forget_last.
+  - rewrite VLSM_weak_stuttering_embedding_finite_trace_last
+      by (eapply valid_trace_forget_last; done).
+    by erewrite finite_valid_trace_from_to_last.
+Qed.
+
+Lemma VLSM_weak_stuttering_embedding_in_futures :
+  forall s1 s2,
+    in_futures X s1 s2 -> in_futures Y (state_project s1) (state_project s2).
+Proof.
+  intros s1 s2 [tr Htr].
+  exists (VLSM_weak_stuttering_embedding_finite_trace_project Hsimul tr).
+  by revert Htr; apply VLSM_weak_stuttering_embedding_finite_valid_trace_from_to.
+Qed.
+
+Lemma VLSM_weak_stuttering_embedding_input_valid_transition_item :
+  forall s item,
+    input_valid_transition_item X s item ->
+    finite_valid_trace_from_to Y (state_project s)
+      (state_project (destination item)) (transition_item_project item).
+Proof.
+  intros.
+  replace (transition_item_project item)
+    with (VLSM_weak_stuttering_embedding_finite_trace_project Hsimul [item])
+    by apply app_nil_r.
+  apply VLSM_weak_stuttering_embedding_finite_valid_trace_from_to.
+  by destruct item; apply finite_valid_trace_from_to_singleton.
+Qed.
+
+End sec_weak_stuttering_embedding_properties.
+
+Section sec_stuttering_embedding_properties.
+
+Context
+  {message : Type}
+  {X Y : VLSM message}
+  {state_project : vstate X -> vstate Y}
+  {transition_item_project : vtransition_item X -> list (vtransition_item Y)}
+  .
+
+Section sec_stuttering_embedding_trace_projection_redefinitions.
+
+(**
+  Here we restate the <<pre_>> definitions above to depend on [VLSM_stuttering_embedding]
+  and have their state and transition item projection functions implicit.
+*)
+
+Definition VLSM_stuttering_embedding_finite_trace_project
+  (Hsimul : VLSM_stuttering_embedding X Y state_project transition_item_project)
+  : list (vtransition_item X) -> list (vtransition_item Y)
+  := pre_VLSM_stuttering_embedding_finite_trace_project transition_item_project.
+
+Definition elem_of_VLSM_stuttering_embedding
+  (Hsimul : VLSM_stuttering_embedding X Y state_project transition_item_project)
+  := elem_of_pre_VLSM_stuttering_embedding_finite_trace_project transition_item_project.
+
+Definition VLSM_stuttering_embedding_infinite_trace_project
+  (Hsimul : VLSM_stuttering_embedding X Y state_project transition_item_project)
+  (s : Streams.Stream (vtransition_item X))
+  (Hinf : InfinitelyOften (fun item => transition_item_project item <> []) s)
+  : Streams.Stream (vtransition_item Y)
+  := pre_VLSM_stuttering_embedding_infinite_trace_project transition_item_project s Hinf.
+
+Definition VLSM_stuttering_embedding_infinite_finite_trace_project
+  (Hsimul : VLSM_stuttering_embedding X Y state_project transition_item_project)
+  (s : Streams.Stream (vtransition_item X))
+  (Hfin : FinitelyManyBound (fun item => transition_item_project item <> []) s)
+  : list (vtransition_item Y)
+  := pre_VLSM_stuttering_embedding_infinite_finite_trace_project transition_item_project s Hfin.
+
+End sec_stuttering_embedding_trace_projection_redefinitions.
+
+(**
+  While for the above section, the [VLSM_stuttering_embedding] was necessary
+  to be mentioned explicitly, in the following we make it part of the context.
+*)
+
+Context
+  (Hsimul : VLSM_stuttering_embedding X Y state_project transition_item_project).
+
+Definition VLSM_stuttering_embedding_finite_trace_project_app :
+  forall l1 l2,
+    VLSM_stuttering_embedding_finite_trace_project Hsimul (l1 ++ l2)
+      =
+    VLSM_stuttering_embedding_finite_trace_project Hsimul l1
+      ++ VLSM_stuttering_embedding_finite_trace_project Hsimul l2
+  := pre_VLSM_stuttering_embedding_finite_trace_project_app transition_item_project.
+
+Definition VLSM_stuttering_embedding_finite_trace_last :
+  forall sX trX,
+    finite_valid_trace_from X sX trX ->
+    finite_trace_last (state_project sX) (VLSM_stuttering_embedding_finite_trace_project Hsimul trX)
+      =
+    state_project (finite_trace_last sX trX)
+  := pre_VLSM_stuttering_embedding_finite_trace_last _ _ _ _ Hsimul.
+
+Definition VLSM_stuttering_embedding_finite_valid_trace :
+  forall sX trX,
+    finite_valid_trace X sX trX -> finite_valid_trace Y (state_project sX)
+      (VLSM_stuttering_embedding_finite_trace_project Hsimul trX)
+  := stuttering_embedding_preserves_valid_trace _ _ _ _ Hsimul.
+
+(**
+  Any [VLSM_stuttering_embedding] determines a [VLSM_partial_projection], allowing us
+  to lift to stuttering embeddings the generic results proved about partial projections.
+*)
+Lemma VLSM_partial_projection_from_stuttering_embedding :
+  VLSM_partial_projection X Y
+    (VLSM_partial_trace_project_from_stuttering_embedding state_project transition_item_project).
+Proof.
+  split.
+  - by apply VLSM_partial_projection_type_from_stuttering_embedding, Hsimul.
+  - intros sX trX sY trY [= <- <-].
+    by apply VLSM_stuttering_embedding_finite_valid_trace.
+Qed.
+
+Lemma VLSM_stuttering_embedding_finite_valid_trace_from :
+  forall sX trX,
+    finite_valid_trace_from X sX trX ->
+    finite_valid_trace_from Y (state_project sX)
+      (VLSM_stuttering_embedding_finite_trace_project Hsimul trX).
+Proof.
+  by intros; eapply VLSM_partial_projection_finite_valid_trace_from;
+    [apply VLSM_partial_projection_from_stuttering_embedding |..].
+Qed.
+
+Definition VLSM_stuttering_embedding_weaken :
+  VLSM_weak_stuttering_embedding X Y state_project transition_item_project :=
+{|
+  weak_stuttering_embedding_type := stuttering_embedding_type _ _ _ _ Hsimul;
+  weak_stuttering_embedding_preserves_valid_trace :=
+    VLSM_stuttering_embedding_finite_valid_trace_from;
+|}.
+
+Definition VLSM_stuttering_embedding_valid_state :
+  forall sX,
+    valid_state_prop X sX -> valid_state_prop Y (state_project sX)
+  := VLSM_weak_stuttering_embedding_valid_state VLSM_stuttering_embedding_weaken.
+
+Definition VLSM_stuttering_embedding_input_valid_transition_item :
+  forall s item,
+    input_valid_transition_item X s item ->
+    finite_valid_trace_from_to Y (state_project s) (state_project (destination item))
+      (transition_item_project item)
+  := VLSM_weak_stuttering_embedding_input_valid_transition_item VLSM_stuttering_embedding_weaken.
+
+Definition VLSM_stuttering_embedding_finite_valid_trace_from_to :
+  forall sX s'X trX,
+    finite_valid_trace_from_to X sX s'X trX ->
+    finite_valid_trace_from_to Y (state_project sX) (state_project s'X)
+      (VLSM_stuttering_embedding_finite_trace_project Hsimul trX)
+  := VLSM_weak_stuttering_embedding_finite_valid_trace_from_to VLSM_stuttering_embedding_weaken.
+
+Definition VLSM_stuttering_embedding_in_futures :
+  forall s1 s2,
+    in_futures X s1 s2 -> in_futures Y (state_project s1) (state_project s2)
+  := VLSM_weak_stuttering_embedding_in_futures VLSM_stuttering_embedding_weaken.
+
+Definition VLSM_stuttering_embedding_infinite_valid_trace_from :
+  forall sX trX (Hinf : InfinitelyOften _ trX),
+    infinite_valid_trace_from X sX trX ->
+    infinite_valid_trace_from Y (state_project sX)
+      (VLSM_stuttering_embedding_infinite_trace_project Hsimul trX Hinf)
+  := VLSM_weak_stuttering_embedding_infinite_valid_trace_from VLSM_stuttering_embedding_weaken.
+
+Definition VLSM_stuttering_embedding_infinite_finite_valid_trace_from :
+  forall sX trX (Hfin : FinitelyManyBound _ trX),
+    infinite_valid_trace_from X sX trX ->
+    finite_valid_trace_from Y (state_project sX)
+      (VLSM_stuttering_embedding_infinite_finite_trace_project Hsimul trX Hfin)
+  := VLSM_weak_stuttering_embedding_infinite_finite_valid_trace_from VLSM_stuttering_embedding_weaken.
+
+Lemma VLSM_stuttering_embedding_initial_state :
+  forall sX, vinitial_state_prop X sX -> vinitial_state_prop Y (state_project sX).
+Proof.
+  by intros; eapply VLSM_partial_projection_initial_state;
+    [apply VLSM_partial_projection_from_stuttering_embedding |..].
+Qed.
+
+Lemma VLSM_stuttering_embedding_finite_valid_trace_init_to :
+  forall sX s'X trX,
+    finite_valid_trace_init_to X sX s'X trX ->
+    finite_valid_trace_init_to Y (state_project sX) (state_project s'X)
+      (VLSM_stuttering_embedding_finite_trace_project Hsimul trX).
+Proof.
+  intros * []; split.
+  - by apply VLSM_stuttering_embedding_finite_valid_trace_from_to.
+  - by apply VLSM_stuttering_embedding_initial_state.
+Qed.
+
+Lemma VLSM_stuttering_embedding_infinite_valid_trace :
+  forall sX trX (Hinf : InfinitelyOften _ trX),
+    infinite_valid_trace X sX trX ->
+    infinite_valid_trace Y (state_project sX)
+      (VLSM_stuttering_embedding_infinite_trace_project Hsimul trX Hinf).
+Proof.
+  intros sX trX Hinf [HtrX HsX].
+  split.
+  - by apply VLSM_stuttering_embedding_infinite_valid_trace_from.
+  - by apply VLSM_stuttering_embedding_initial_state.
+Qed.
+
+Lemma VLSM_stuttering_embedding_infinite_finite_valid_trace :
+  forall sX trX (Hfin : FinitelyManyBound _ trX),
+    infinite_valid_trace X sX trX ->
+    finite_valid_trace Y (state_project sX)
+      (VLSM_stuttering_embedding_infinite_finite_trace_project Hsimul trX Hfin).
+Proof.
+  intros sX trX Hfin [HtrX HsX].
+  split.
+  - by apply VLSM_stuttering_embedding_infinite_finite_valid_trace_from.
+  - by apply VLSM_stuttering_embedding_initial_state.
+Qed.
+
+(** ** Stuttering embedding friendliness
+
+  A stuttering embedding is friendly if all the valid traces of the destination VLSM
+  are prefixes of translations of the valid traces of the source VLSM.
+*)
+
+Section sec_stuttering_embedding_friendliness.
+
+(**
+  We axiomatize stuttering embedding friendliness as the converse of
+  [VLSM_stuttering_embedding_finite_valid_trace]. However, since a transition
+  in the source corresponds to possibly multiple transitions in the destination,
+  we'll ask that any valid trace in the destination is the prefix of a
+  translation of a valid trace from the source.
+*)
+Definition stuttering_embedding_friendly_prop : Prop :=
+  forall
+    (sY : vstate Y)
+    (trY : list (vtransition_item Y))
+    (HtrY : finite_valid_trace Y sY trY),
+  exists (sX : vstate X) (trX : list (vtransition_item X)),
+    finite_valid_trace X sX trX
+    /\ state_project sX = sY
+    /\ trY `prefix_of` VLSM_stuttering_embedding_finite_trace_project Hsimul trX.
+
+Lemma stuttering_embedding_friendly_finite_valid_trace_from_to
+  (Hfr : stuttering_embedding_friendly_prop)
+  (sY1 sY2 : vstate Y) (trY : list (vtransition_item Y))
+  (HtrY : finite_valid_trace_from_to Y sY1 sY2 trY)
+  : exists (sX1 sX2 : vstate X) (trX : list (vtransition_item X))
+      (preY sufY : list (vtransition_item Y)),
+      finite_valid_trace_from_to X sX1 sX2 trX /\
+      VLSM_stuttering_embedding_finite_trace_project Hsimul trX = preY ++ trY ++ sufY.
+Proof.
+  apply finite_valid_trace_from_to_complete_left in HtrY
+    as (is & tr_s1 & Htr & _).
+  apply valid_trace_forget_last, Hfr in Htr as [isX [trX [[Htr _] [His [suf Htr_pr]]]]].
+  exists isX, (finite_trace_last isX trX), trX, tr_s1, suf.
+  split.
+  - by apply valid_trace_add_default_last.
+  - by rewrite app_assoc.
+Qed.
+
+(**
+  A consequence of the [stuttering_embedding_friendly_prop]erty is that the valid
+  traces of the target VLSM are precisely prefixes of translations of all
+  the valid traces of the source VLSM.
+*)
+Lemma stuttering_embedding_friendly_trace_char
+  (Hfriendly : stuttering_embedding_friendly_prop)
+  : forall sY trY, finite_valid_trace Y sY trY <->
+    exists (sX : vstate X) (trX : list (vtransition_item X)),
+    finite_valid_trace X sX trX
+    /\ state_project sX = sY
+    /\ trY `prefix_of` VLSM_stuttering_embedding_finite_trace_project Hsimul trX.
+Proof.
+  split; [by apply Hfriendly |].
+  intros (sX & trX & HtrX & <- & sufY & HtrY).
+  apply VLSM_stuttering_embedding_finite_valid_trace in HtrX as [HtrX].
+  split; [| done].
+  eapply finite_valid_trace_from_app_iff.
+  by rewrite <- HtrY.
+Qed.
+
+End sec_stuttering_embedding_friendliness.
+
+End sec_stuttering_embedding_properties.
+
+(**
+  To establish a stuttering embedding from VLSM <<X>> to VLSM <<Y>>,
+  the following set of conditions is sufficient:
+  - <<X>>'s [initial_state]s project to <<Y>>'s [initial state]s
+  - Every input-valid transition translates to a valid trace from the translation
+    of the source of the transition to the translation of the destination
+    of the transition
+*)
+
+Section sec_basic_VLSM_stuttering_embedding.
+
+Section sec_strong_VLSM_stuttering_embedding_type.
+
+Context
+  {message : Type}
+  (X : VLSM message)
+  (TY : VLSMType message)
+  (state_project : vstate X -> @state _ TY)
+  (transition_item_project : vtransition_item X -> list (@transition_item _ TY))
+  .
+
+Lemma strong_VLSM_stuttering_embedding_type
+  (Htransition : strong_transition_item_project_consistency state_project transition_item_project)
+  : VLSM_stuttering_embedding_type X TY state_project transition_item_project.
+Proof. by constructor; intros ? [] []; apply Htransition. Qed.
+
+End sec_strong_VLSM_stuttering_embedding_type.
+
+Context
+  {message : Type}
+  (X Y : VLSM message)
+  (state_project : vstate X -> vstate Y)
+  (transition_item_project : vtransition_item X -> list (vtransition_item Y))
+  (Htransition : stuttering_embedding_input_valid_transition_item_validity
+    X Y state_project transition_item_project)
+  .
+
+Lemma basic_VLSM_stuttering_embedding_type :
+  VLSM_stuttering_embedding_type X (type Y) state_project transition_item_project.
+Proof.
+  constructor; intros.
+  by eapply finite_valid_trace_from_to_last, Htransition.
+Qed.
+
+Section sec_weak_stuttering_embedding.
+
+Context
+  (Hstate : weak_stuttering_embedding_initial_state_preservation X Y state_project)
+  .
+
+#[local] Lemma basic_VLSM_stuttering_embedding_finite_valid_trace_init_to
+  is s tr
+  (Htr : finite_valid_trace_init_to X is s tr)
+  : finite_valid_trace_from_to Y (state_project is) (state_project s)
+      (pre_VLSM_stuttering_embedding_finite_trace_project transition_item_project tr).
+Proof.
+  induction Htr using finite_valid_trace_init_to_rev_ind; [by constructor; apply Hstate |].
+  rewrite pre_VLSM_stuttering_embedding_finite_trace_project_app.
+  apply finite_valid_trace_from_to_app with (state_project s); [done |].
+  cbn; rewrite app_nil_r.
+  remember {| l := _|} as itemX; replace sf with (destination itemX) by (subst; done).
+  by apply Htransition; subst.
+Qed.
+
+#[local] Lemma basic_VLSM_stuttering_embedding_finite_valid_trace_from
+  (s : state)
+  (ls : list transition_item)
+  (Hpxt : finite_valid_trace_from X s ls)
+  : finite_valid_trace_from Y (state_project s)
+      (pre_VLSM_stuttering_embedding_finite_trace_project transition_item_project ls).
+Proof.
+  apply valid_trace_add_default_last,
+    finite_valid_trace_from_to_complete_left
+    in Hpxt as (is_s & tr_s & Htr & Heqs).
+  replace (state_project s) with
+    (finite_trace_last (state_project is_s)
+      (pre_VLSM_stuttering_embedding_finite_trace_project transition_item_project tr_s)).
+  - eapply valid_trace_forget_last, finite_valid_trace_from_to_app_split.
+    rewrite <- pre_VLSM_stuttering_embedding_finite_trace_project_app.
+    by apply basic_VLSM_stuttering_embedding_finite_valid_trace_init_to.
+  - subst s; apply pre_VLSM_stuttering_embedding_finite_trace_last.
+    + by apply basic_VLSM_stuttering_embedding_type.
+    + by eapply valid_trace_forget_last, finite_valid_trace_from_to_app_split, Htr.
+Qed.
+
+Lemma basic_VLSM_weak_stuttering_embedding :
+  VLSM_weak_stuttering_embedding X Y state_project transition_item_project.
+Proof.
+  constructor.
+  - by apply basic_VLSM_stuttering_embedding_type.
+  - by apply basic_VLSM_stuttering_embedding_finite_valid_trace_from.
+Qed.
+
+End sec_weak_stuttering_embedding.
+
+Lemma basic_VLSM_weak_stuttering_embedding_strengthen
+  (Hweak : VLSM_weak_stuttering_embedding X Y state_project transition_item_project)
+  (Hstate : strong_stuttering_embedding_initial_state_preservation X Y state_project)
+  : VLSM_stuttering_embedding X Y state_project transition_item_project.
+Proof.
+  constructor; [by apply Hweak |].
+  intros sX trX [HtrX HsX].
+  split.
+  - by apply (VLSM_weak_stuttering_embedding_finite_valid_trace_from Hweak).
+  - by apply Hstate.
+Qed.
+
+Lemma basic_VLSM_stuttering_embedding
+  (Hstate : strong_stuttering_embedding_initial_state_preservation X Y state_project)
+  : VLSM_stuttering_embedding X Y state_project transition_item_project.
+Proof.
+  apply basic_VLSM_weak_stuttering_embedding_strengthen; [| done].
+  apply basic_VLSM_weak_stuttering_embedding.
+  by apply strong_stuttering_embedding_initial_state_preservation_weaken.
+Qed.
+
+End sec_basic_VLSM_stuttering_embedding.
