theories/VLSM/Lib/NeList.v
@@ -1,0 +1,251 @@
+From stdpp Require Import prelude.
+From VLSM.Lib Require Import ListExtras StdppExtras.
+
+(** A straight-forward inductive definition of non-empty lists. *)
+Inductive ne_list (A : Type) : Type :=
+| nel_singl : A -> ne_list A
+| nel_cons : A -> ne_list A -> ne_list A.
+
+Arguments nel_singl  {_} _ : assert.
+Arguments nel_cons {_} _ _ : assert.
+
+Infix ":::" := nel_cons (at level 60, right associativity).
+
+Definition ne_list_hd {A} (l : ne_list A) : A :=
+  match l with
+  | nel_singl a => a
+  | nel_cons a _ => a
+  end.
+
+Definition ne_list_tl {A} (l : ne_list A) : option (ne_list A) :=
+  match l with
+  | nel_singl _ => None
+  | nel_cons _ tl => Some tl
+  end.
+
+Definition ne_list_foldr {A B} (f : A -> B -> B) (b : B) (l : ne_list A) :=
+  (fix fold (l : ne_list A) :=
+    match l with
+    | nel_singl a => f a b
+    | nel_cons a tl => f a (fold tl)
+    end) l.
+
+Definition ne_list_app {A} (l1 l2 : ne_list A) := ne_list_foldr nel_cons l2 l1.
+
+#[export] Instance ne_list_ret : MRet ne_list := @nel_singl.
+
+#[export] Instance ne_list_bind : MBind ne_list :=
+  fun A B f l => (fix bind (l : ne_list A) :=
+    match l with
+    | nel_singl a => f a
+    | nel_cons a tl => ne_list_app (f a) (bind tl)
+    end) l.
+
+#[export] Instance ne_list_fmap  : FMap ne_list :=
+  fun A B f => mbind (mret ∘ f).
+
+#[export] Instance ne_list_join : MJoin ne_list :=
+  fun A => mbind id.
+
+Inductive ne_list_equiv `{Equiv A} : Equiv (ne_list A) :=
+| ne_one_equiv x y : x ≡ y -> nel_singl x ≡ nel_singl y
+| ne_cons_equiv x y l k : x ≡ y → l ≡ k → x ::: l ≡ y ::: k.
+
+#[export] Existing Instance ne_list_equiv.
+
+Definition ne_list_to_list {A} (nel : ne_list A) : list A :=
+  ne_list_foldr cons [] nel.
+
+Definition ne_list_length {A} (nel : ne_list A) := length (ne_list_to_list nel).
+
+Lemma ne_list_min_length {A} (nel : ne_list A) : 1 <= ne_list_length nel.
+Proof. by destruct nel; cbn; lia. Qed.
+
+Lemma ne_list_to_list_unroll {A} (a : A) (tl : ne_list A) :
+  ne_list_to_list (a ::: tl) = a :: ne_list_to_list tl.
+Proof. done. Qed.
+
+Definition ne_list_to_list_tl {A} (l : ne_list A) : list A :=
+  match l with
+  | nel_singl _ => []
+  | nel_cons _ tl => ne_list_to_list tl
+  end.
+
+Definition ne_list_option_cons {A} (a : A) (mnel : option (ne_list A)) : ne_list A :=
+  from_option (nel_cons a) (nel_singl a) mnel.
+
+Definition list_to_option_ne_list {A} (l : list A) : option (ne_list A) :=
+  foldr (fun a mnel => Some (ne_list_option_cons a mnel)) None l.
+
+Lemma list_to_option_ne_list_unroll {A} (a : A) l :
+  list_to_option_ne_list (a :: l) = Some (ne_list_option_cons a (list_to_option_ne_list l)).
+Proof. done. Qed.
+
+(** A definition of non-empty lists based on lists. *)
+Record NeList (A : Type) : Type :=
+{
+  nl_hd : A;
+  nl_tl : list A;
+}.
+
+Arguments nl_hd {_} _ : assert.
+Arguments nl_tl {_} _ : assert.
+
+Definition ne_list_to_NeList {A} (l : ne_list A) : NeList A :=
+{|
+  nl_hd := ne_list_hd l;
+  nl_tl := ne_list_to_list_tl l;
+|}.
+
+Definition NeList_to_ne_list {A} (l : NeList A) : ne_list A :=
+  ne_list_option_cons (nl_hd l) (list_to_option_ne_list (nl_tl l)).
+
+Lemma NeList_to_ne_list_unroll {A} (a b : A) (l : list A) :
+  NeList_to_ne_list {| nl_hd := a; nl_tl := b :: l |}
+    =
+  nel_cons a (NeList_to_ne_list {| nl_hd := b; nl_tl := l|}).
+Proof. done. Qed.
+
+Lemma NeList_to_ne_list_to_list {A} :
+  forall (l : NeList A),
+    ne_list_to_list (NeList_to_ne_list l) = nl_hd l :: nl_tl l.
+Proof.
+  intros [h t]; revert h; induction t; intros; [done |].
+  by rewrite NeList_to_ne_list_unroll, ne_list_to_list_unroll, IHt.
+Qed.
+
+Lemma NeList_to_ne_list_to_NeList {A} :
+  forall (l : NeList A),
+    ne_list_to_NeList (NeList_to_ne_list l) = l.
+Proof.
+  intros [h1 [| h2 t]]; [done |].
+  rewrite NeList_to_ne_list_unroll.
+  unfold ne_list_to_NeList; f_equal.
+  by apply NeList_to_ne_list_to_list.
+Qed.
+
+Lemma ne_list_to_list_to_nelist {A} :
+  forall (l : ne_list A),
+    list_to_option_ne_list (ne_list_to_list l) = Some l.
+Proof.
+  induction l; [done |].
+  rewrite ne_list_to_list_unroll, list_to_option_ne_list_unroll.
+  by rewrite IHl.
+Qed.
+
+Lemma ne_list_to_NeList_to_ne_list {A} :
+  forall (l : ne_list A),
+    NeList_to_ne_list (ne_list_to_NeList l) = l.
+Proof.
+  intros [a | a n]; [done |].
+  unfold ne_list_to_NeList, NeList_to_ne_list, nl_hd, nl_tl, ne_list_hd, ne_list_to_list_tl.
+  by rewrite ne_list_to_list_to_nelist.
+Qed.
+
+#[export] Instance elem_of_ne_list {A} : ElemOf A (ne_list A) :=
+  fun a nel => a ∈ ne_list_to_list nel.
+
+#[export] Instance ne_list_subseteq {A} : SubsetEq (ne_list A) :=
+  fun l1 l2 => forall x, x ∈ l1 → x ∈ l2.
+
+#[export] Instance elem_of_ne_list_dec `{dec : EqDecision A} :
+  RelDecision (∈@{ne_list A}).
+Proof.
+  intros a l.
+  unfold elem_of, elem_of_ne_list; cbn.
+  by typeclasses eauto.
+Qed.
+
+Definition ne_list_from_non_empty_list {A} (l : list A) : l <> [] -> ne_list A :=
+  match l with
+  | [] => fun H => False_rect _ (H eq_refl)
+  | a :: l' => fun _ => NeList_to_ne_list {| nl_hd := a; nl_tl := l' |}
+  end.
+
+Definition list_function_restriction {A B} (f : A -> list B)
+  (da : dsig (fun a => f a <> [])) : ne_list B :=
+  ne_list_from_non_empty_list (f (` da)) (proj2_dsig da).
+
+Lemma list_filter_map_mbind
+  {A B : Type}
+  (f : A -> list B)
+
+  (l : list A)
+  : mjoin (map ne_list_to_list
+      (list_filter_map (fun a => f a <> []) (list_function_restriction f) l))
+    = mbind f l.
+Proof.
+  induction l using rev_ind; [done |].
+  rewrite mbind_app, list_filter_map_app, map_app, mjoin_app, IHl.
+  cbn; clear IHl.
+  f_equal; rewrite app_nil_r.
+  destruct (decide _) as [Hfx | Hnfx]; cbn;
+    [| by destruct (decide (f x = []))].
+  unfold list_function_restriction, ne_list_from_non_empty_list; cbn in Hfx.
+  remember (proj2_dsig _) as Hp; clear HeqHp; cbn in Hp.
+  simpl.
+  destruct (f x); [done |].
+  by rewrite NeList_to_ne_list_to_list, app_nil_r.
+Qed.
+
+Lemma ne_list_concat_min_length
+  {A : Type}
+  (l : list (ne_list A))
+  : length (mjoin (map ne_list_to_list l)) >= length l.
+Proof.
+  induction l; cbn; [by lia |].
+  rewrite app_length.
+  (* by specialize (ne_list_min_length a); unfold ne_list_length; lia. *)
+  (* for some strange reason the line above does not work, so... this hack: *)
+  assert (Hle : forall a b c, a >= 1 -> b >= c -> a + b >= S c) by lia.
+  by apply Hle; [apply ne_list_min_length |].
+Qed.
+
+(**
+  An alternative inductive definition of non-empty lists using a single
+  constructor.
+*)
+Inductive NonEmptyList (A : Type) : Type := NEL_cons
+{
+  nel_hd : A;
+  nel_tl : option (NonEmptyList A)
+}.
+
+Arguments nel_hd {_} _ : assert.
+Arguments nel_tl {_} _ : assert.
+Arguments NEL_cons {_} _ _ : assert.
+
+#[export] Instance NonEmptyList_inhabited `{Inhabited A} : Inhabited (NonEmptyList A) :=
+  populate (NEL_cons inhabitant None).
+
+Definition NEL_singl `(a : A) : NonEmptyList A := NEL_cons a None.
+
+Fixpoint NonEmptyList_ind'
+  (A : Type) (P : NonEmptyList A -> Prop)
+  (hd' : forall h : A, P (NEL_cons h None))
+  (tl' : forall (h : A) (t : NonEmptyList A), P t -> P (NEL_cons h (Some t)))
+  (l : NonEmptyList A) {struct l} : P l :=
+match l with
+| NEL_cons h None => hd' h
+| NEL_cons h (Some t) => tl' h t (NonEmptyList_ind' A P hd' tl' t)
+end.
+
+Fixpoint NonEmptyList_to_ne_list `(l : NonEmptyList A) : ne_list A :=
+  match nel_tl l with
+  | None => nel_singl (nel_hd l)
+  | Some l' => nel_cons (nel_hd l) (NonEmptyList_to_ne_list l')
+  end.
+
+Fixpoint ne_list_to_NonEmptyList `(l : ne_list A) : NonEmptyList A :=
+  match l with
+  | nel_singl a => NEL_singl a
+  | nel_cons a l' => NEL_cons a (Some (ne_list_to_NonEmptyList l'))
+  end.
+
+Lemma NonEmptyList_to_ne_list_to_NonEmptyList `(l : NonEmptyList A) :
+  ne_list_to_NonEmptyList (NonEmptyList_to_ne_list l) = l.
+Proof. by induction l using NonEmptyList_ind'; cbn; [| rewrite IHl]. Qed.
+
+Lemma ne_list_to_NonEmptyList_to_ne_list `(l : ne_list A) :
+  NonEmptyList_to_ne_list (ne_list_to_NonEmptyList l) = l.
+Proof. by induction l; cbn; [| rewrite IHl]. Qed.
